Logically atomic refactoring of the lazy list proof

lazy_list/code.v
@@ -1,11 +1,34 @@
 From iris.heap_lang Require Export notation spin_lock.
 
-From SkipList.lib Require Import node_rep.
 
+Section node_rep.
+  Definition node_rep : Type := Z * loc * val.
+  Definition dummy_null : loc := {|loc_car := 0|}.
+  Definition dummy_lock : val := #().
 
-Local Open Scope Z.
+  Definition node_key (n: node_rep) : Z := n.1.1.
+  Definition node_next (n: node_rep) : loc := n.1.2.
+  Definition node_lock (n: node_rep) : val := n.2.
+
+  Definition nodeKey : val := λ: "l", Fst (Fst "l").
+  Definition nodeNext : val := λ: "l", Snd (Fst "l").
+  Definition nodeLock : val := λ: "l", Snd "l".
+
+  Definition rep_to_node (n: node_rep) : val :=
+    (#(node_key n), #(node_next n), (node_lock n)).
+  Lemma fold_rep_to_node (n: node_rep) :
+    ((#(node_key n), #(node_next n), (node_lock n)))%V = rep_to_node n.
+  Proof. done. Qed.
+  Lemma rep_to_node_inj rep rep':
+    rep_to_node rep = rep_to_node rep' → rep = rep'.
+  Proof.
+    destruct rep as ((?&?)&?); destruct rep' as ((?&?)&?). 
+    rewrite /rep_to_node/node_key/node_next/node_lock/=; congruence.
+  Qed.
+End node_rep.
 
 Module Type LAZY_LIST_PARAMS.
+  Local Open Scope Z.
   Parameter INT_MIN : Z.
   Parameter INT_MAX : Z.
   Parameter (HMIN_MAX: INT_MIN < INT_MAX).
@@ -14,12 +37,12 @@ End LAZY_LIST_PARAMS.
 Module LazyList (Params: LAZY_LIST_PARAMS).
   Import Params.
   
-  Definition tail : node_rep := (INT_MAX, dummy_null, dummy_null, None, dummy_lock, dummy_null).  
+  Definition tail : node_rep := (INT_MAX, dummy_null, dummy_lock).  
 
   Definition new : val := 
     λ: "_", 
       let: "t" := ref (rep_to_node tail) in
-        ref (#INT_MIN, #dummy_null, "t", NONEV, newlock #(), #dummy_null).
+        ref (#INT_MIN, "t", newlock #()).
 
   Definition find : val := 
     rec: "find" "pred" "k" :=
@@ -49,11 +72,12 @@ Module LazyList (Params: LAZY_LIST_PARAMS).
       let: "pair" := findLock !"p" "k" in
       let: "pred" := Fst "pair" in
       let: "succ" := Snd "pair" in
+      let: "lock" := nodeLock "pred" in
         if: "k" = nodeKey "succ"
-        then release (nodeLock "pred")
+        then release "lock"
         else let: "np" := nodeNext "pred" in
              let: "next" := ref !"np" in
-               "np" <- ("k", #dummy_null, "next", NONEV, newlock #(), #dummy_null);;
-               release (nodeLock "pred").
+               "np" <- ("k", "next", newlock #());;
+               release "lock".
 
 End LazyList.
