jelly_fish/code.v
@@ -1,0 +1,189 @@
+From iris.heap_lang Require Export notation spin_lock.
+
+
+Local Open Scope Z.
+
+Section node_rep.
+  Definition node_rep : Type := Z * loc * loc * loc.
+  Definition dummy_null : loc := {|loc_car := 0|}.
+
+  Definition node_key (n: node_rep) : Z := n.1.1.1.
+  Definition node_val (n: node_rep) : loc := n.1.1.2.
+  Definition node_next (n: node_rep) : loc := n.1.2.
+  Definition node_lock (n: node_rep) : loc := n.2.
+
+  Definition nodeKey : val := λ: "l", Fst (Fst (Fst "l")).
+  Definition nodeVal : val := λ: "l", Snd (Fst (Fst "l")).
+  Definition nodeNext : val := λ: "l", Snd (Fst "l").
+  Definition nodeLock : val := λ: "l", Snd "l".
+
+  Definition rep_to_node (n: node_rep) : val :=
+    (#(node_key n), #(node_val n), #(node_next n), #(node_lock n)).
+  Lemma fold_rep_to_node (n: node_rep) :
+    ((#(node_key n), #(node_val n), #(node_next n), #(node_lock n)))%V = rep_to_node n.
+  Proof. done. Qed.
+  Lemma rep_to_node_inj rep rep':
+    rep_to_node rep = rep_to_node rep' → rep = rep'.
+  Proof.
+    destruct rep as (((?&?)&?)&?); destruct rep' as (((?&?)&?)&?). 
+    rewrite /rep_to_node/node_key/node_val/node_next/node_lock/=; congruence.
+  Qed.
+End node_rep.
+
+Section val_rep.
+  Definition val_rep : Type := Z * Z * loc.
+  Definition dummy_val : val_rep := (0, 0, dummy_null).
+
+  Definition val_v (v: val_rep) : Z := v.1.1.
+  Definition val_t (v: val_rep) : Z := v.1.2.
+  Definition val_p (v: val_rep) : loc := v.2.
+
+  Definition valV : val := λ: "l", Fst (Fst "l").
+  Definition valT : val := λ: "l", Snd (Fst "l").
+  Definition valP : val := λ: "l", Snd "l".
+
+  Definition rep_to_val (v: val_rep) : val := 
+    (#(val_v v), #(val_t v), #(val_p v)).
+  Lemma fold_rep_to_val (v: val_rep) :
+    ((#(val_v v), #(val_t v), #(val_p v)))%V =
+    rep_to_val v.
+  Proof. done. Qed.
+  Lemma rep_to_val_inj rep rep' :
+    rep_to_val rep = rep_to_val rep' →
+    rep = rep'.
+  Proof.
+    destruct rep as ((?&?)&?); destruct rep' as ((?&?)&?).
+    rewrite /rep_to_val/val_v/val_t/val_p/=; congruence.
+  Qed.
+End val_rep.
+
+Module Type SKIP_LIST_PARAMS.
+  Parameter INT_MIN : Z.
+  Parameter INT_MAX : Z.
+  Parameter MAX_HEIGHT : Z.
+  Parameter (HMIN_MAX: INT_MIN < INT_MAX).
+  Parameter (HMAX_HEIGHT: 0 ≤ MAX_HEIGHT).
+End SKIP_LIST_PARAMS.
+
+Module SkipList (Params: SKIP_LIST_PARAMS).
+  Import Params.
+  
+  Definition tail : node_rep := (INT_MAX, dummy_null, dummy_null, dummy_null).
+
+  Definition initLocks : val := 
+    rec: "init" "locks" "lvl" :=
+      if: "lvl" = #(MAX_HEIGHT + 1) then #()
+      else "locks" +ₗ "lvl" <- newlock #();;
+           "init" "locks" ("lvl" + #1).
+
+  Definition new : val := 
+    λ: "_", 
+      let: "nexts" := AllocN #(MAX_HEIGHT + 1) (ref (rep_to_node tail)) in
+      let: "locks" := AllocN #(MAX_HEIGHT + 1) #() in
+        initLocks "locks" #0;;
+        ref (#INT_MIN, #dummy_null, "nexts", "locks").
+
+  Definition find : val := 
+    rec: "find" "pred" "k" "lvl" :=
+      let: "succ" := ! !(nodeNext "pred" +ₗ "lvl") in
+        if: "k" ≤ nodeKey "succ" then ("pred", "succ")
+        else "find" "succ" "k" "lvl".
+  
+  Definition findLock : val := 
+    rec: "find" "pred" "k" "lvl" :=
+      let: "pair" := find "pred" "k" "lvl" in
+      let: "pred" := Fst "pair" in
+      let: "lock" := !(nodeLock "pred" +ₗ "lvl") in
+        acquire "lock";;
+        let: "succ" := ! !(nodeNext "pred" +ₗ "lvl") in
+          if: "k" ≤ nodeKey "succ" then ("pred", "succ")
+          else release "lock";;
+               "find" "succ" "k" "lvl".
+
+  Definition findAll : val := 
+    rec: "find" "pred" "k" "lvl" "h" := 
+      let: "pair" := find "pred" "k" "lvl" in
+      let: "pred" := Fst "pair" in
+        if: "lvl" = "h" then "pair"
+        else "find" "pred" "k" ("lvl" - #1) "h".
+
+  Definition get : val :=
+    λ: "p" "k", 
+      let: "pair" := findAll !"p" "k" #MAX_HEIGHT #0 in
+      let: "succ" := Snd "pair" in
+        if: "k" ≠ nodeKey "succ" then NONEV
+        else let: "val" := !(nodeVal "succ") in SOME (valV "val", valT "val").
+
+  Definition link : val := 
+    λ: "pred" "lvl" "n",
+      let: "new" := !"n" in
+        nodeNext "new" +ₗ "lvl" <- !(nodeNext "pred" +ₗ "lvl") ;;
+        nodeLock "new" +ₗ "lvl" <- newlock #();;
+        nodeNext "pred" +ₗ "lvl" <- "n".
+
+  Definition insert : val := 
+    λ: "pred" "lvl" "n",
+      let: "k" := nodeKey !"n" in
+      let: "pair" := findLock "pred" "k" "lvl" in
+      let: "pred" := Fst "pair" in
+      let: "lock" := !(nodeLock "pred" +ₗ "lvl") in
+        link "pred" "lvl" "n";;
+        release "lock".
+
+  Definition createAndLink : val := 
+    λ: "pred" "k" "v" "t" "h",
+      let: "nexts" := AllocN ("h" + #1) #() in
+      let: "locks" := AllocN ("h" + #1) #() in
+      let: "val" := ref ("v", "t", #dummy_null) in
+      let: "n" := ref ("k", "val", "nexts", "locks") in
+        link "pred" #0 "n";;
+        "n".
+
+  Definition update : val := 
+    λ: "node" "v" "t",
+      let: "val" := !(nodeVal "node") in
+        if: "t" < valT "val" then #()
+        else nodeVal "node" <- ("v", "t", ref "val").
+
+  Definition tryInsert : val := 
+    λ: "pred" "k" "v" "t" "h",
+      let: "pair" := findLock "pred" "k" #0 in
+      let: "pred" := Fst "pair" in
+      let: "succ" := Snd "pair" in
+      let: "lock" := !(nodeLock "pred") in
+        if: "k" = nodeKey "succ"
+        then update "succ" "v" "t";;
+             release "lock";;
+             NONEV
+        else let: "n" := createAndLink "pred" "k" "v" "t" "h" in
+               release "lock";;
+               SOME "n".
+
+  Definition insertAll : val := 
+    rec: "insert" "curr" "k" "v" "t" "h" "lvl" := 
+      if: "lvl" = #0 then tryInsert "curr" "k" "v" "t" "h"
+      else let: "pair" := find "curr" "k" ("lvl" - #1) in
+           let: "pred" := Fst "pair" in
+           let: "opt" := "insert" "pred" "k" "v" "t" "h" ("lvl" - #1) in
+             match: "opt" with
+               NONE => NONEV
+             | SOME "n" => insert "curr" "lvl" "n";;
+                           SOME "n"
+             end.
+
+  Definition putH : val := 
+    λ: "p" "k" "v" "t" "h",
+      let: "pair" := findAll !"p" "k" #MAX_HEIGHT "h" in
+      let: "pred" := Fst "pair" in
+        insertAll "pred" "k" "v" "t" "h" "h".
+
+  (* HeapLang does not support randomness... *)
+  Definition randomLevel : val :=
+    λ: "_", #0.
+
+  Definition put : val :=
+    λ: "p" "k" "v" "t",
+      let: "h" := randomLevel #() in
+      let: "_" := putH "p" "k" "v" "t" "h" in #().
+
+End SkipList.
