jelly_fish/inv/lazy_inv.v
@@ -1,0 +1,60 @@
+From Coq Require Import Sorting.Sorted.
+
+From iris.base_logic.lib Require Import invariants.
+From iris.algebra Require Import cmra auth frac_auth gmap gset.
+From iris.heap_lang Require Import proofmode.
+
+From SkipList.lib Require Import arg_max.
+From SkipList.jelly_fish Require Import code.
+From SkipList.lib Require Import misc node_rep node_lt.
+From SkipList.jelly_fish Require Import list_equiv.
+
+Module LazyListInv (Params: SKIP_LIST_PARAMS).
+  Import Params.
+  Module ListEquiv := ListEquiv Params.
+  Export ListEquiv.
+
+  Section Proofs.
+    Context `{!heapGS Σ, !skipGS Σ, !lockG Σ} (lvl: Z).
+
+    Definition opt_map (osub: option sub_gname) (M: gmap Z (argmax Z)) : option (gmap Z (argmax Z)) :=
+      match osub with
+      | Some _ => None
+      | None => Some M
+      end.
+
+    Definition sub_list_inv (head: node_rep) (Γ: sub_gname) (osub: option sub_gname) 
+      (M: gmap Z (argmax Z)) (S: gset node_rep) (L: list node_rep) : iProp Σ := 
+      ⌜ Permutation L (elements S) ⌝
+      ∗
+      ⌜ Sorted node_lt ([head] ++ L ++ [tail]) ⌝
+      ∗
+      own (s_auth Γ) (● S)
+      ∗
+      own (s_toks Γ) (● GSet (set_map node_key S))
+      ∗
+      list_equiv lvl osub ([head] ++ L) (opt_map osub M).
+
+    Definition lazy_list_inv (head: node_rep) (obot: option bot_gname)
+      (Γ: sub_gname) (osub: option sub_gname) : iProp Σ := 
+        ∃ (M: gmap Z (argmax Z)) (S: gset node_rep) (L: list node_rep),
+          sub_list_inv head Γ osub M S L
+          ∗
+          match obot with
+          | Some bot => own (s_frac bot) (●F M) ∗ ⌜ dom M = set_map node_key S ⌝
+          | None => True
+          end.
+
+    Definition levelN (lvl: Z) := nroot .@ "level" .@ lvl.
+
+    Definition is_sub_list (head: node_rep) (Γ γ: sub_gname) : iProp Σ := 
+      inv (levelN lvl) (lazy_list_inv head None Γ (Some γ)).
+
+    Definition is_bot_list (head: node_rep) (M: gmap Z (argmax Z)) (q: frac)
+      (bot: bot_gname) (Γ: sub_gname) : iProp Σ := 
+      own (s_frac bot) (◯F{q} M)
+      ∗
+      inv (levelN lvl) (lazy_list_inv head (Some bot) Γ None).
+
+  End Proofs.
+End LazyListInv.
