jelly_fish/spec/new.v
@@ -1,0 +1,191 @@
+From iris.base_logic.lib Require Import invariants.
+From iris.algebra Require Import auth frac_auth gmap gset.
+From iris.heap_lang Require Import proofmode.
+
+From SkipList.lib Require Import arg_max.
+From SkipList.jelly_fish Require Import code.
+From SkipList.lib Require Import misc node_rep node_lt.
+From SkipList.jelly_fish.inv Require Import list_equiv lazy_inv skip_inv.
+
+
+Local Open Scope Z.
+
+Module NewSpec (Params: SKIP_LIST_PARAMS).
+  Import Params.
+  Module Invariant := SkipListInv Params.
+  Export Invariant.
+
+  Section Proofs.
+    Context `{!heapGS Σ, !skipGS Σ, !lockG Σ}.
+
+    Theorem initLocks_spec (lvl: Z) (head: node_rep) (t: loc)
+      (bot: bot_gname) (subs: list sub_gname) :
+      {{{
+        skip_list_equiv (lvl - 1) head ∅ 1 bot subs
+        ∗
+        t ↦□ rep_to_node tail
+        ∗
+        (node_next head +ₗ lvl) ↦∗ replicate (Z.to_nat (MAX_HEIGHT + 1 - lvl)) #t
+        ∗
+        (node_locks head +ₗ lvl) ↦∗ replicate (Z.to_nat (MAX_HEIGHT + 1 - lvl)) #()
+        ∗
+        ⌜ 1 ≤ lvl ≤ MAX_HEIGHT + 1 ⌝ 
+        ∗
+        ⌜ node_key head = INT_MIN ⌝ 
+      }}}
+        initLocks #(node_locks head) #lvl
+      {{{ subs, RET #();
+        skip_list_equiv MAX_HEIGHT head ∅ 1 bot subs
+      }}}.
+    Proof.
+      iIntros (Φ) "(Hskip & #Ht & Hnext & Hlocks & Hlvl & %Hmin) HΦ".
+      iRevert (lvl subs) "Hskip Hnext Hlocks Hlvl HΦ".
+      iLöb as "IH".
+      iIntros (lvl subs) "Hskip Hnext Hlocks %Hlvl HΦ".
+
+      wp_lam. wp_let. wp_pures.
+      case_bool_decide as Hcase; wp_if.
+      + iModIntro; iApply ("HΦ" $! subs).
+        inversion Hcase; subst.
+        by assert (MAX_HEIGHT + 1 - 1 = MAX_HEIGHT) as -> by lia.
+      + assert (lvl ≠ MAX_HEIGHT + 1) as Hneq by congruence.
+        destruct subs as [|γ subs]; first by iExFalso.
+
+        assert (Z.to_nat (MAX_HEIGHT + 1 - lvl) = S (Z.to_nat (MAX_HEIGHT - lvl))) as -> by lia.
+        repeat rewrite replicate_S array_cons.
+        iDestruct "Hlocks" as "(Hl & Hlocks)".
+        iDestruct "Hnext" as "((Hnext' & Hnext'') & Hnext)".
+
+        wp_apply (newlock_spec (in_lock lvl (Some γ) head) with "[Hnext'']").
+        { iExists t; iFrame. }
+        iIntros (l γl) "#Hlock".
+
+        wp_store. wp_pures.
+        iMod (mapsto_persist with "Hl") as "#Hl".
+
+        iMod (own_alloc (● ∅ ⋅ ◯ ∅))
+          as (γauth) "[Hown_auth _]"; 
+          first by apply auth_both_valid.
+        iMod (own_alloc (● GSet ∅ ⋅ ◯ GSet ∅))
+          as (γtoks) "[Hown_toks _]"; 
+          first by apply auth_both_valid.
+
+        set (Γ := mk_sub_gname γauth γtoks).
+        iMod (inv_alloc (levelN lvl) ⊤ (lazy_list_inv lvl head None Γ (Some γ)) 
+          with "[Hnext' Hown_auth Hown_toks]") as "Hinv".
+        {
+          iNext; iExists ∅, ∅, nil.
+          rewrite /sub_list_inv set_map_empty.
+          iFrame. iSplit; first done. 
+          iSplit.
+          {
+            assert (node_lt head tail); last (simpl; auto).
+            rewrite /node_key in Hmin.
+            rewrite /node_lt /node_key Hmin /=; apply HMIN_MAX.
+          }
+          iExists γl, l, t; iFrame "# ∗".
+        }
+
+        iApply ("IH" $! _ (Γ :: γ :: subs) with "[Hskip Hinv] [Hnext] [Hlocks] [%]").
+        {
+          assert (lvl + 1 - 1 = lvl) as -> by lia.
+          iFrame. iPureIntro; lia.
+        }
+        {
+          assert (MAX_HEIGHT + 1 - (lvl + 1) = MAX_HEIGHT - lvl) as -> by lia.
+          rewrite -loc_add_assoc //.
+        }
+        {
+          assert (MAX_HEIGHT + 1 - (lvl + 1) = MAX_HEIGHT - lvl) as -> by lia.
+          rewrite -loc_add_assoc //.
+        }
+        { lia. }
+
+        iNext; done.
+    Qed.
+
+    Theorem new_spec : 
+      {{{ True }}}
+        new #()
+      {{{ p bot subs, RET #p; is_skip_list p ∅ 1 bot subs }}}.
+    Proof.
+      iIntros (Φ) "_ HΦ".
+      pose proof HMAX_HEIGHT as Hmax.
+
+      wp_lam. 
+      wp_alloc t as "Ht"; iMod (mapsto_persist with "Ht") as "#Ht".
+      wp_alloc next as "Hnext"; first lia. wp_let.
+      wp_alloc locks as "Hlocks"; first lia. wp_let.
+
+      assert (Z.to_nat (MAX_HEIGHT + 1) = S (Z.to_nat MAX_HEIGHT)) as -> by lia.
+      rewrite replicate_S ?array_cons.
+      iDestruct "Hnext" as "((Hn & Hn') & Hnext)".
+      iDestruct "Hlocks" as "(Hlocks' & Hlocks)".
+
+      wp_lam. wp_let. wp_pures.
+      case_bool_decide as Hcase; first (inversion Hcase; lia).
+      wp_if.
+
+      set (head := (INT_MIN, dummy_null, next, @None loc, dummy_lock, locks)).
+      wp_apply (newlock_spec (in_lock 0 None head) with "[Hn']").
+      { 
+        iExists t; rewrite loc_add_0; iFrame.
+        iExists tail; iFrame "#"; by iLeft.
+      }
+      iIntros (l γl) "#Hlock".
+
+      wp_pures; rewrite loc_add_0.
+      wp_store; iMod (mapsto_persist with "Hlocks'") as "#Hl".
+      wp_pures; assert (0 + 1 = 1) as -> by lia.
+
+      iMod (own_alloc (● ∅ ⋅ ◯ ∅))
+        as (γauth) "[Hown_auth _]"; 
+        first by apply auth_both_valid.
+      iMod (own_alloc (● GSet ∅ ⋅ ◯ GSet ∅))
+        as (γtoks) "[Hown_toks _]"; 
+        first by apply auth_both_valid.
+      iMod (own_alloc (●F (∅ : gmap Z (argmax Z)) ⋅ ◯F (∅: gmap Z (argmax Z))))
+        as (γfrac) "[Hown_frac Hown_frac_frag]"; 
+        first by apply auth_both_valid.
+
+      set (Γ := mk_sub_gname γauth γtoks).
+      set (bot := mk_bot_gname γfrac).
+      iMod (inv_alloc (levelN 0) ⊤ (lazy_list_inv 0 head (Some bot) Γ None) 
+        with "[Hn Hown_auth Hown_toks Hown_frac]") as "Hinv".
+      {
+        iNext; iExists ∅, ∅, nil. 
+        rewrite /sub_list_inv set_map_empty dom_empty_L.
+        iFrame. iSplit; last done. iSplit; first done. 
+        iSplit.
+        {
+          assert (node_lt head tail); last (simpl; auto).
+          rewrite /node_lt/node_key//=; apply HMIN_MAX.
+        }
+
+        iExists γl, l, t.
+        repeat rewrite loc_add_0.
+        iFrame "# ∗".
+      }
+
+      iAssert (skip_list_equiv 0 head ∅ 1 bot [Γ]) 
+        with "[Hinv Hown_frac_frag]" as "Hskip".
+      { by iFrame. }
+
+      assert (locks = node_locks head) as Hlocks by auto; rewrite Hlocks.
+      wp_apply (initLocks_spec 1 head t with "[Hskip Hlocks Hnext]").
+      {
+        assert (MAX_HEIGHT + 1 - 1 = MAX_HEIGHT) as -> by lia.
+        assert (1 - 1 = 0) as -> by lia.
+        iFrame "# ∗". iPureIntro.
+        by split; first lia.
+      }
+      iIntros (subs) "Hskip". wp_pures.
+      rewrite (fold_rep_to_node head).
+
+      wp_alloc p as "Hp"; iMod (mapsto_persist with "Hp") as "#Hp".
+      iModIntro; iApply ("HΦ" $! p bot subs).
+      iExists head. by iFrame "# ∗".
+    Qed.
+
+  End Proofs.
+End NewSpec.
