lazy_list/client/rw_example.v
@@ -1,0 +1,84 @@
+From iris.algebra Require Import gset.
+From iris.program_logic Require Import atomic.
+From iris.heap_lang Require Import par proofmode.
+
+From SkipList.lazy_list Require Import code.
+From SkipList.lazy_list.client Require Import rw_spec.
+
+
+Module Params <: LAZY_LIST_PARAMS.
+  Local Open Scope Z.
+  Definition INT_MIN := -1000.
+  Definition INT_MAX := 1000.
+  Lemma HMIN_MAX : INT_MIN < INT_MAX.
+  Proof. unfold INT_MIN, INT_MAX; lia. Qed.
+End Params.
+
+Module Import Spec := RWSpec Params.
+
+Definition exampleN := nroot .@ "example".
+
+Definition lazy_list_client : expr := 
+  let: "p" := new #() in
+    ((add "p" #0;; add "p" #1) ||| (add "p" #1;; add "p" #2));;
+    (contains "p" #2 ||| contains "p" #0).
+
+Section Proofs.
+  Context `{!heapGS Σ, !rwG Σ, !spawnG Σ}.
+
+  Lemma lazy_list_client_spec :
+    {{{ True }}}
+      lazy_list_client
+    {{{ RET (#true, #true); True }}}.
+  Proof.
+    iIntros (Φ) "_ HΦ".
+
+    unfold lazy_list_client.
+    wp_apply (new_spec exampleN); first done.
+    iIntros (p Γs) "(#Hset_inv & Hset)".
+    iDestruct (rw_inv_alloc_mut exampleN with "Hset") as ">Hinv".
+    iDestruct "Hinv" as (Γ) "(#Hinv & Hmut)".
+
+    wp_let. 
+    rewrite -(Qp.div_2 1); iDestruct (mut_set_sep with "Hmut") as "(Hmut1 & Hmut2)".
+    wp_smart_apply (wp_par (λ _, mut_set _ _ _) (λ _, mut_set _ _ _) with "[Hmut1] [Hmut2]").
+    {
+      awp_apply (write_spec with "Hinv Hset_inv"); first rewrite /Params.INT_MIN/Params.INT_MAX//.
+      iAaccIntro with "Hmut1"; first (iIntros "?"; iModIntro; iFrame).
+      iIntros "Hmut1"; iModIntro; wp_pures.
+
+      awp_apply (write_spec with "Hinv Hset_inv"); first rewrite /Params.INT_MIN/Params.INT_MAX//.
+      iAaccIntro with "Hmut1"; first (iIntros "?"; iModIntro; iFrame).
+      iIntros "?"; iModIntro; rewrite left_id_L //.
+    }
+    { 
+      awp_apply (write_spec with "Hinv Hset_inv"); first rewrite /Params.INT_MIN/Params.INT_MAX//.
+      iAaccIntro with "Hmut2"; first (iIntros "?"; iModIntro; iFrame).
+      iIntros "Hmut2"; iModIntro; wp_pures.
+
+      awp_apply (write_spec with "Hinv Hset_inv"); first rewrite /Params.INT_MIN/Params.INT_MAX//.
+      iAaccIntro with "Hmut2"; first (iIntros "?"; iModIntro; iFrame).
+      iIntros "?"; iModIntro; rewrite left_id_L //.
+    }
+    
+    iIntros (? ?) "Hmut"; iDestruct (mut_set_join with "Hmut") as "Hmut".
+    iNext; wp_pure; wp_pure.
+    rewrite gset_op Qp.div_2; iDestruct (mut_to_const with "Hinv Hmut") as ">Hconst".
+    rewrite -(Qp.div_2 1); iDestruct (const_set_sep with "Hconst") as "(Hconst1 & Hconst2)".
+    wp_smart_apply (wp_par (λ v, ⌜ v = #true ⌝%I) (λ v, ⌜ v = #true ⌝%I) with "[Hconst1] [Hconst2]").
+    {
+      awp_apply (read_spec with "Hinv Hset_inv"); first rewrite /Params.INT_MIN/Params.INT_MAX//.
+      iAaccIntro with "Hconst1"; first (iIntros "?"; iModIntro; iFrame).
+      iIntros (b) "(_ & %Hif)"; iModIntro; iPureIntro.
+      destruct (b); first done; last set_solver.
+    }
+    {
+      awp_apply (read_spec with "Hinv Hset_inv"); first rewrite /Params.INT_MIN/Params.INT_MAX//.
+      iAaccIntro with "Hconst2"; first (iIntros "?"; iModIntro; iFrame).
+      iIntros (b) "(_ & %Hif)"; iModIntro; iPureIntro.
+      destruct (b); first done; last set_solver.
+    }
+
+    iIntros (? ?) "(-> & ->)"; iNext; by iApply "HΦ".
+  Qed.
+End Proofs.
