lazy_list/client/rw_spec.v
@@ -1,0 +1,181 @@
+From iris.algebra Require Import gset frac_auth.
+From iris.base_logic.lib Require Import invariants.
+From iris.program_logic Require Import atomic.
+From iris.heap_lang Require Import proofmode.
+
+From SkipList.lazy_list Require Import code inv.
+From SkipList.lazy_list.spec Require Import spec.
+
+
+Class rwG Σ := RWG { 
+  rw_mutG :> inG Σ (frac_authR (gsetR Z));
+  rw_agrG :> inG Σ (frac_authR (agreeR (gset Z)));
+  rw_setG :> lazyG Σ
+}.
+
+Record rw_gname := mk_rw_gname {
+  mut_gname: gname;
+  agr_gname: gname
+}.
+
+Module RWSpec (Params: LAZY_LIST_PARAMS).
+  Import Params.
+  Module LASpec := LASpec Params.
+  Export LASpec.
+
+  Section invariant.
+    Context `{!heapGS Σ, !rwG Σ} (N: namespace).
+
+    Definition rw_lazyN := N .@ "rw_lazy".
+
+    (* Public state for concurrent writes *)
+    Definition mut_set (s: gset Z) (q: frac) (Γ: rw_gname) : iProp Σ := 
+      own Γ.(mut_gname) (◯F{q} s).
+    Lemma mut_set_sep s q1 q2 Γ :
+      mut_set s (q1 + q2) Γ -∗ mut_set s q1 Γ ∗ mut_set s q2 Γ.
+    Proof. iIntros "(Hmut1 & Hmut2)"; iFrame. Qed.
+    Lemma mut_set_join s1 s2 q1 q2 Γ :
+      mut_set s1 q1 Γ ∗ mut_set s2 q2 Γ -∗ mut_set (s1 ⋅ s2) (q1 + q2) Γ.
+    Proof. iIntros "(Hmut1 & Hmut2)"; by iCombine "Hmut1 Hmut2" as "Hmut". Qed.
+
+    (* Public state for concurrent reads *)
+    Definition const_set (s: gset Z) (q: frac) (Γ: rw_gname) : iProp Σ := 
+      own Γ.(agr_gname) (◯F{q} (to_agree s)).
+    Lemma const_set_sep s q1 q2 Γ :
+      const_set s (q1 + q2) Γ -∗ const_set s q1 Γ ∗ const_set s q2 Γ.
+    Proof. iIntros "(Hmut1 & Hmut2)"; iFrame. Qed.
+    Lemma const_set_join s1 s2 q1 q2 Γ :
+      const_set s1 q1 Γ ∗ const_set s2 q2 Γ -∗ const_set (s1 ⋅ s2) (q1 + q2) Γ.
+    Proof. 
+      iIntros "(Hmut1 & Hmut2)"; iCombine "Hmut1 Hmut2" as "Hmut". 
+      iDestruct (own_valid with "Hmut") as %[_ <-%to_agree_op_inv_L]%frac_auth_frag_valid.
+      rewrite gset_op union_idemp_L agree_idemp //.
+    Qed.
+
+    (* Invariant concealing the abstract state of the full set *)
+    Definition rw_inv (Γ: rw_gname) (Γs: set_gname) : iProp Σ :=
+      ∃ (s: gset Z),
+        set s Γs
+        ∗
+        own Γ.(mut_gname) (●F s)
+        ∗
+        own Γ.(agr_gname) (●F (to_agree s))
+        ∗
+        (own Γ.(mut_gname) (◯F s) ∨ own Γ.(agr_gname) (◯F (to_agree s))).
+    Lemma rw_inv_alloc_mut s Γs:
+      set s Γs ={⊤}=∗ ∃ Γ, inv rw_lazyN (rw_inv Γ Γs) ∗ mut_set s 1 Γ.
+    Proof.
+      iIntros "Hset".
+      iMod (own_alloc (●F s ⋅ ◯F s)) as (γmut) "[Hmut● Hmut◯]"; 
+        first by apply auth_both_valid.
+      iMod (own_alloc (●F (to_agree s) ⋅ ◯F (to_agree s))) as (γagr) "[Hagr● Hagr◯]"; 
+        first by apply auth_both_valid.
+      set (Γ := mk_rw_gname γmut γagr).
+      iMod (inv_alloc rw_lazyN ⊤ (rw_inv Γ Γs) 
+        with "[Hset Hmut● Hagr● Hagr◯]") as "#Hinv".
+      { iNext; iExists s; iFrame. }
+      iModIntro; iExists Γ; iFrame "# ∗".
+    Qed.
+    Lemma rw_inv_alloc_const s Γs:
+      set s Γs ={⊤}=∗ ∃ Γ, inv rw_lazyN (rw_inv Γ Γs) ∗ const_set s 1 Γ.
+    Proof.
+      iIntros "Hset".
+      iMod (own_alloc (●F s ⋅ ◯F s)) as (γmut) "[Hmut● Hmut◯]"; 
+        first by apply auth_both_valid.
+      iMod (own_alloc (●F (to_agree s) ⋅ ◯F (to_agree s))) as (γagr) "[Hagr● Hagr◯]"; 
+        first by apply auth_both_valid.
+      set (Γ := mk_rw_gname γmut γagr).
+      iMod (inv_alloc rw_lazyN ⊤ (rw_inv Γ Γs) 
+        with "[Hset Hmut● Hmut◯ Hagr●]") as "#Hinv".
+      { iNext; iExists s; iFrame. }
+      iModIntro; iExists Γ; iFrame "# ∗".
+    Qed.
+
+    (* Helper lemmas for switching between concurrent writes and concurrent reads *)
+    Lemma mut_to_const s Γ Γs :
+      inv rw_lazyN (rw_inv Γ Γs) -∗ mut_set s 1 Γ ={⊤}=∗ const_set s 1 Γ.
+    Proof.
+      rewrite /mut_set/const_set; iIntros "#Hinv Hmut◯".
+      iInv "Hinv" as (s') ">(Hset & Hmut● & Hagr● & Hagr◯)".
+      iDestruct (own_valid_2 with "Hmut● Hmut◯") as %->%frac_auth_agree_L.
+      iDestruct "Hagr◯" as "[Hfalse|Hagr◯]".
+      { by iDestruct (own_valid_2 with "Hmut◯ Hfalse") as %[Hfalse%Qp.not_add_le_r _]%frac_auth_frag_valid. }
+      iModIntro. iSplitR "Hagr◯"; last (iModIntro; iFrame).
+      iNext; iExists s; iFrame.
+    Qed.
+    Lemma const_to_mut s Γ Γs :
+      inv rw_lazyN (rw_inv Γ Γs) -∗ const_set s 1 Γ ={⊤}=∗ mut_set s 1 Γ.
+    Proof.
+      rewrite /mut_set/const_set; iIntros "#Hinv Hagr◯".
+      iInv "Hinv" as (s') ">(Hset & Hmut● & Hagr● & Hmut◯)".
+      iDestruct (own_valid_2 with "Hagr● Hagr◯") as %Heq%frac_auth_agree.
+      replace s' with s by rewrite -to_agree_op_valid_L Heq agree_idemp //.
+      iDestruct "Hmut◯" as "[Hmut◯|Hfalse]"; last first.
+      { by iDestruct (own_valid_2 with "Hagr◯ Hfalse") as %[Hfalse%Qp.not_add_le_r _]%frac_auth_frag_valid. }
+      iModIntro. iSplitR "Hmut◯"; last (iModIntro; iFrame).
+      iNext; iExists s; iFrame.
+    Qed.
+  End invariant.
+
+  Section proofs.
+    Context `{!heapGS Σ, !rwG Σ} (N: namespace).
+    Local Open Scope Z.
+
+    Theorem read_spec (p: loc) (Γ: rw_gname) (Γs: set_gname)
+      (k: Z) (Hrange: INT_MIN < k < INT_MAX) :
+      inv (rw_lazyN N) (rw_inv Γ Γs) -∗
+      set_inv N p Γs -∗
+      <<< ∀∀ (s: gset Z) (q: frac), const_set s q Γ >>>
+        contains #p #k @ ↑N
+      <<< ∃∃ (b: bool), const_set s q Γ ∗ ⌜ if b then k ∈ s else k ∉ s ⌝, RET #b >>>.
+    Proof.
+      iIntros "#Hinv #Hset_inv %Φ AU"; rewrite /const_set.
+
+      awp_apply (contains_spec with "Hset_inv"); first done.
+      iInv "Hinv" as (s) ">(Hset & Hmut● & Hagr● & Hmut◯)".
+      iApply (aacc_aupd with "AU"). 
+      { rewrite difference_difference_l; apply difference_mono_l, union_least; apply nclose_subseteq. }
+      iIntros (s' q) "Hagr◯"; iAaccIntro with "Hset".
+      { do 2 (iIntros "?"; iModIntro; iFrame); iNext; iExists s; iFrame. }
+      iIntros (b) "(Hset & Hif)".
+
+      iDestruct (own_valid_2 with "Hagr● Hagr◯") as %Heq%frac_auth_included.
+      rewrite Some_included_total to_agree_included leibniz_equiv_iff in Heq; rewrite Heq.
+
+      iModIntro; iRight; iExists b; iFrame.
+      iIntros "?"; iModIntro; iFrame.
+      iNext; iExists s; iFrame.
+    Qed.
+
+    Theorem write_spec (p: loc) (Γ: rw_gname) (Γs: set_gname)
+      (k: Z) (Hrange: INT_MIN < k < INT_MAX) :
+      inv (rw_lazyN N) (rw_inv Γ Γs) -∗
+      set_inv N p Γs -∗
+      <<< ∀∀ (s: gset Z) (q: frac), mut_set s q Γ >>>
+        add #p #k @ ↑N
+      <<< mut_set (s ⋅ {[ k ]}) q Γ, RET #() >>>.
+    Proof.
+      iIntros "#Hinv #Hset_inv %Φ AU"; rewrite /const_set.
+
+      awp_apply (add_spec with "Hset_inv"); first done.
+      iInv "Hinv" as (s) ">(Hset & Hmut● & Hagr● & Hagr◯)".
+      iApply (aacc_aupd with "AU"). 
+      { rewrite difference_difference_l; apply difference_mono_l, union_least; apply nclose_subseteq. }
+      iIntros (s' q) "Hmut◯"; iAaccIntro with "Hset".
+      { do 2 (iIntros "?"; iModIntro; iFrame); iNext; iExists s; iFrame. }
+      iIntros "Hset".
+
+      iMod (own_update_2 with "Hmut● Hmut◯") as "[Hmut● Hmut◯]".
+      { by apply frac_auth_update, (op_local_update_discrete _ _ {[k]}). }
+      do 2 rewrite (comm _ {[k]} _) gset_op.
+      iDestruct "Hagr◯" as "[Hfalse|Hagr◯]".
+      { by iDestruct (own_valid_2 with "Hmut◯ Hfalse") as %[Hfalse%Qp.not_add_le_r _]%frac_auth_frag_valid. }
+      iMod (own_update_2 with "Hagr● Hagr◯") as "[Hagr● Hagr◯]".
+      { by apply (frac_auth_update_1 _ _ (to_agree (s ∪ {[k]}))). }
+
+      iModIntro; iRight; iFrame.
+      iIntros "?"; iModIntro; iFrame.
+      iNext; iExists (s ∪ {[k]}); iFrame.
+    Qed.
+  End proofs.
+End RWSpec.
