lazy_list/inv.v
@@ -1,0 +1,87 @@
+From iris.algebra Require Import gset excl_auth.
+From iris.base_logic.lib Require Import invariants.
+From iris.heap_lang Require Import proofmode.
+
+From SkipList.lib Require Import zrange.
+From SkipList.lazy_list Require Import code.
+
+
+Class lazyG Σ := LazyG { 
+  lazy_authG :> inG Σ (authR (gsetR node_rep));
+  lazy_disjG :> inG Σ (gset_disjR Z);
+  lazy_exclG :> inG Σ (excl_authR (gset Z));
+  lazy_lockG :> lockG Σ
+}.
+
+Record inv_gname := mk_inv_gname {
+  auth_gname: gname;
+  disj_gname: gname
+}.
+
+Record set_gname := mk_set_gname {
+  excl_gname: gname
+}.
+
+Module LazyListInv (Params: LAZY_LIST_PARAMS).
+  Import Params.
+  Module LazyList := LazyList Params.
+  Export LazyList.
+
+  Section invariant.
+    Context `{!heapGS Σ, !lazyG Σ} (N: namespace).
+
+    Definition lazyN := N .@ "lazy".
+
+    Definition in_lock (l: loc) : iProp Σ := 
+      ∃ (succ: node_rep), l ↦{#1 / 2} rep_to_node succ.
+
+    Definition has_lock (node: node_rep) : iProp Σ := 
+      ∃ (γl: gname), is_lock γl (node_lock node) (in_lock (node_next node)).
+
+    Definition has_next (Γi: inv_gname) (pred: node_rep) : iProp Σ :=
+      ∃ (succ: node_rep), 
+        node_next pred ↦{#1 / 2} rep_to_node succ
+        ∗
+        (⌜ succ = tail ⌝ ∨ own Γi.(auth_gname) (◯ {[succ]}))
+        ∗
+        own Γi.(disj_gname) (ZRange (node_key pred) (node_key succ)).
+
+    Definition lazy_list_inv (head: node_rep) (Γi: inv_gname) (Γs: set_gname) : iProp Σ :=
+      ∃ (S: gset node_rep),
+        own Γi.(auth_gname) (● S)
+        ∗
+        own Γi.(disj_gname) (GSet (set_map node_key S))
+        ∗
+        ([∗ set] n ∈ {[head]} ∪ S, has_lock n)
+        ∗
+        ([∗ set] n ∈ {[head]} ∪ S, has_next Γi n)
+        ∗
+        own Γs.(excl_gname) (●E (set_map node_key S)).
+
+    Definition set_inv (p: loc) (Γs: set_gname) : iProp Σ :=
+      ∃ (head: node_rep) (Γi: inv_gname),
+        p ↦□ rep_to_node head
+        ∗
+        ⌜ node_key head = INT_MIN ⌝
+        ∗
+        inv lazyN (lazy_list_inv head Γi Γs).
+
+    Definition set (s: gset Z) (Γs: set_gname) : iProp Σ := 
+      own Γs.(excl_gname) (◯E s).
+
+  End invariant.
+
+  Section proofs.
+    Context `{!lazyG Σ}.
+
+    Lemma singleton_frag_in S n s Γ :
+      own Γ (● S) -∗ ⌜ n = s ⌝ ∨ own Γ (◯ {[n]}) -∗ ⌜ n ∈ {[s]} ∪ S ⌝.
+    Proof.
+      iIntros "Hauth Hnode".
+      iDestruct "Hnode" as "[->|Hnode]"; first (iPureIntro; set_solver).
+      iDestruct (own_valid_2 with "Hauth Hnode") 
+        as %[?%gset_included]%auth_both_valid_discrete.
+      iPureIntro; set_solver.
+    Qed.
+  End proofs.
+End LazyListInv.
