lazy_list/spec/find.v
@@ -1,0 +1,201 @@
+From iris.algebra Require Import gset excl_auth.
+From iris.base_logic.lib Require Import invariants.
+From iris.program_logic Require Import atomic.
+From iris.heap_lang Require Import proofmode.
+
+From SkipList.lib Require Import zrange.
+From SkipList.lazy_list Require Import code inv.
+
+
+Module FindSpec (Params: LAZY_LIST_PARAMS).
+  Import Params.
+  Module Invariant := LazyListInv Params.
+  Export Invariant.
+
+  Section proofs.
+    Context `{!heapGS Σ, !lazyG Σ} (N: namespace).
+    Local Open Scope Z.
+    
+    Theorem find_spec (k: Z) (head curr: node_rep) (Γi: inv_gname) (Γs: set_gname) :
+      node_key curr < k < INT_MAX →
+      inv (lazyN N) (lazy_list_inv head Γi Γs) -∗
+      (⌜ curr = head ⌝ ∨ own Γi.(auth_gname) (◯ {[curr]})) -∗
+      <<< ∀∀ (s: gset Z), own Γs.(excl_gname) (◯E s) >>>
+        find (rep_to_node curr) #k @ ↑(lazyN N)
+      <<< ∃∃ pred succ,
+        own Γs.(excl_gname) (◯E s)
+        ∗
+        ⌜ k ∈ s ↔ node_key succ = k ⌝
+        ∗
+        (⌜ pred = head ⌝ ∨ own Γi.(auth_gname) (◯ {[pred]}))
+        ∗
+        (⌜ succ = tail ⌝ ∨ own Γi.(auth_gname) (◯ {[succ]}))
+        ∗
+        ⌜ node_key pred < k ≤ node_key succ ⌝
+        ∗
+        ∃ (γl: gname), is_lock γl (node_lock pred) (in_lock (node_next pred)),
+      RET ((rep_to_node pred), (rep_to_node succ)) >>>.
+    Proof.
+      iIntros "%Hk #Hinv Hcurr %Φ"; iRevert (curr Hk) "Hcurr".
+      iLöb as "IH"; iIntros "%curr %Hk #Hcurr AU".
+      wp_lam. wp_let. wp_lam. wp_pures.
+
+      wp_bind (Load _).
+      iInv "Hinv" as (S) "(>Hauth & >Hdisj & Hlocks & Hnexts & >Hexcl●)".
+
+      iDestruct (singleton_frag_in with "Hauth Hcurr") as %Hcurr.
+      rewrite (big_sepS_delete has_lock _ curr) // (big_sepS_delete (has_next _) _ curr) //.
+      iDestruct "Hlocks" as "(Hlock & Hlocks)"; iDestruct "Hnexts" as "(Hnext & Hnexts)".
+      iDestruct "Hlock" as (γl) "#His_lock"; iDestruct "Hnext" as (succ) ">(Hnext & #Hsucc & Hkeys)".
+
+      destruct (decide(k ≤ node_key succ)) as [|Hcase].
+      + iMod "AU" as (?) "[Hexcl◯ [_ Hclose]]".
+        iDestruct (own_valid_2 with "Hexcl● Hexcl◯") as %<-%excl_auth_agree_L.
+        iDestruct (own_valid_2 with "Hdisj Hkeys") as %[Hdisj _]%ZRange_disj.
+        iDestruct (singleton_frag_in with "Hauth Hsucc") as %Hsucc%elem_of_union.
+        rewrite elem_of_singleton in Hsucc.
+
+        wp_load.
+        iAssert (has_lock curr) as "Hlock".
+        { iExists γl; iFrame "#". }
+        iAssert (has_next _ curr) with "[Hnext Hkeys]" as "Hnext".
+        { iExists succ; by iFrame. }
+        iCombine "Hlock Hlocks" as "Hlocks"; iCombine "Hnext Hnexts" as "Hnexts".
+        do 2 rewrite -big_sepS_delete //.
+
+        iDestruct ("Hclose" with "[Hexcl◯]") as ">HΦ"; last iModIntro.
+        {
+          iFrame "# ∗"; iPureIntro.
+          split; last lia; split.
+          + intros Hin; destruct (decide (node_key succ = k)); first done.
+            exfalso. rewrite zrange_disj in Hdisj; apply (Hdisj k); first lia; done.
+          + intros <-; destruct Hsucc as [->|Hsucc]; last set_solver.
+            exfalso. rewrite /node_key/= in Hk; lia.
+        }
+
+        iModIntro; iSplitL "Hauth Hdisj Hlocks Hnexts Hexcl●".
+        { iNext; iExists S; by iFrame. }
+        wp_let; wp_lam; wp_pures.
+
+        case_bool_decide; last lia; wp_if.
+        by wp_pure.
+      + wp_load.
+        iAssert (has_lock curr) as "Hlock".
+        { iExists γl; iFrame "#". }
+        iAssert (has_next _ curr) with "[Hnext Hkeys]" as "Hnext".
+        { iExists succ; by iFrame. }
+        iCombine "Hlock Hlocks" as "Hlocks"; iCombine "Hnext Hnexts" as "Hnexts".
+        do 2 rewrite -big_sepS_delete //.
+
+        iModIntro; iSplitL "Hauth Hdisj Hlocks Hnexts Hexcl●".
+        { iNext; iExists S; by iFrame. }
+        wp_let; wp_lam; wp_pures.
+
+        case_bool_decide; first lia; wp_if.
+        iDestruct "Hsucc" as "[->|Hsucc]"; first (rewrite /node_key/= in Hcase; lia).
+        iApply ("IH" with "[%] [$] AU"); lia.
+    Qed.
+
+    Theorem find_lock_spec (k: Z) (head curr: node_rep) (Γi: inv_gname) (Γs: set_gname) :
+      node_key curr < k < INT_MAX →
+      inv (lazyN N) (lazy_list_inv head Γi Γs) -∗
+      (⌜ curr = head ⌝ ∨ own Γi.(auth_gname) (◯ {[curr]})) -∗
+      <<< ∀∀ (s: gset Z), own Γs.(excl_gname) (◯E s) >>>
+        findLock (rep_to_node curr) #k @ ↑(lazyN N)
+      <<< ∃∃ pred succ,
+        own Γs.(excl_gname) (◯E s)
+        ∗
+        ⌜ k ∈ s ↔ node_key succ = k ⌝
+        ∗
+        (⌜ pred = head ⌝ ∨ own Γi.(auth_gname) (◯ {[pred]}))
+        ∗
+        (⌜ succ = tail ⌝ ∨ own Γi.(auth_gname) (◯ {[succ]}))
+        ∗
+        ⌜ node_key pred < k ≤ node_key succ ⌝
+        ∗
+        ∃ (γl: gname), is_lock γl (node_lock pred) (in_lock (node_next pred))
+                      ∗
+                      node_next pred ↦{#1 / 2} rep_to_node succ
+                      ∗
+                      locked γl,
+      RET ((rep_to_node pred), (rep_to_node succ)) >>>.
+    Proof.
+      iIntros "%Hk #Hinv Hcurr %Φ"; iRevert (curr Hk) "Hcurr".
+      iLöb as "IH"; iIntros (curr Hk) "#Hcurr AU".
+      wp_lam. wp_let.
+      
+      awp_apply (find_spec with "Hinv Hcurr"); first done.
+      iApply (aacc_aupd with "AU"); first done.
+      iIntros (s) "Hexcl◯"; iAaccIntro with "Hexcl◯".
+      { do 2 (iIntros "?"; iModIntro; iFrame). }
+      iIntros (pred succ') "(Hexcl◯ & _ & #Hpred & _ & (%Hk' & _) & His_lock)".
+      iDestruct "His_lock" as (γl) "#His_lock".
+
+      iModIntro; iLeft; iFrame. 
+      iIntros "AU"; iModIntro.
+      wp_pures; wp_lam; wp_pures.
+
+      wp_bind (acquire _).
+      iApply (acquire_spec with "His_lock").
+      iNext; iIntros "(Hlocked & Hin_lock)".
+      iDestruct "Hin_lock" as (succ) "Hnext'".
+      wp_pures; wp_lam; wp_pures.
+
+      wp_bind (Load _). 
+      iInv "Hinv" as (S) "(>Hauth & >Hdisj & Hlocks & Hnexts & >Hexcl●)".
+
+      iDestruct (singleton_frag_in with "Hauth Hpred") as %Hpred.
+      rewrite (big_sepS_delete (has_next _) _ pred) //.
+      iDestruct "Hnexts" as "(Hnext & Hnexts)".
+      iDestruct "Hnext" as (?) ">(Hnext & #Hsucc & Hkeys)".
+      iDestruct (mapsto_agree with "Hnext Hnext'") as %->%rep_to_node_inj.
+
+      destruct (decide(k ≤ node_key succ)) as [|Hcase].
+      + iMod "AU" as (?) "[Hexcl◯ [_ Hclose]]".
+        iDestruct (own_valid_2 with "Hexcl● Hexcl◯") as %<-%excl_auth_agree_L.
+        iDestruct (own_valid_2 with "Hdisj Hkeys") as %[Hdisj _]%ZRange_disj.
+        iDestruct (singleton_frag_in with "Hauth Hsucc") as %Hsucc%elem_of_union.
+        rewrite elem_of_singleton in Hsucc.
+
+        wp_load.
+        iAssert (has_next _ pred) with "[Hnext Hkeys]" as "Hnext".
+        { iExists succ; by iFrame. }
+        iCombine "Hnext Hnexts" as "Hnexts".
+        rewrite -big_sepS_delete //.
+
+        iDestruct ("Hclose" with "[Hexcl◯ Hlocked Hnext']") as ">HΦ"; last iModIntro.
+        {
+          iFrame "# ∗". iSplit; first last.
+          { iSplit; first (iPureIntro; lia). iExists γl; iFrame "# ∗". }
+          iPureIntro; split.
+          - intros Hin; destruct (decide (node_key succ = k)); first done.
+            exfalso. rewrite zrange_disj in Hdisj; apply (Hdisj k); first lia; done.
+          - intros <-; destruct Hsucc as [->|Hsucc]; last set_solver.
+            exfalso. rewrite /node_key/= in Hk; lia.
+        }
+
+        iModIntro; iSplitL "Hauth Hdisj Hlocks Hnexts Hexcl●".
+        { iNext; iExists S; by iFrame. }
+        wp_let; wp_lam; wp_pures.
+
+        case_bool_decide; last lia; wp_if.
+        by wp_pure.
+      + wp_load.
+        iAssert (has_next _ pred) with "[Hnext Hkeys]" as "Hnext".
+        { iExists succ; by iFrame. }
+        iCombine "Hnext Hnexts" as "Hnexts".
+        rewrite -big_sepS_delete //.
+
+        iModIntro; iSplitL "Hauth Hdisj Hlocks Hnexts Hexcl●".
+        { iNext; iExists S; by iFrame. }
+        wp_let; wp_lam; wp_pures.
+
+        case_bool_decide; first lia; wp_if.
+        wp_apply (release_spec with "[Hlocked Hnext']").
+        { iFrame "# ∗"; iExists succ; iFrame. }
+        iIntros "_"; wp_pures.
+        iDestruct "Hsucc" as "[->|Hsucc]"; first (rewrite /node_key/= in Hcase; lia).
+        iApply ("IH" with "[%] [$] AU"); lia.
+    Qed.
+  End proofs.
+End FindSpec.
