lib/gmap_extra.v
@@ -1,0 +1,37 @@
+From iris.algebra Require Import gmap.
+
+
+Section extra.
+  Context `{Countable K} {A : cmra}.
+  Implicit Types m : gmap K A.
+  Implicit Types i : K.
+  Implicit Types x y : A.
+
+  Lemma insert_singleton_op_Some m i x y : 
+    m !! i = Some x → <[i:=y ⋅ x]> m ≡ {[ i := y ]} ⋅ m.
+  Proof.
+    intros Hsome; symmetry.
+    rewrite -(insert_delete m i x) //.
+    rewrite insert_singleton_op; last apply lookup_delete.
+    rewrite assoc singleton_op.
+    do 2 (rewrite -insert_singleton_op; last apply lookup_delete).
+    rewrite (insert_delete m i x) //.
+    by rewrite insert_delete_insert.
+  Qed.
+
+  Lemma insert_singleton_op_Some_L `{!LeibnizEquiv A} m i x y : 
+    m !! i = Some x → <[i:=y ⋅ x]> m = {[ i := y ]} ⋅ m.
+  Proof. intros; rewrite -leibniz_equiv_iff insert_singleton_op_Some //. Qed.  
+
+  Lemma insert_singleton_op_empty i x : 
+    <[i:=x]> (∅ : gmap K A) = {[ i := x ]} ⋅ ∅.
+  Proof. by apply insert_singleton_op. Qed.
+
+  Lemma dom_singleton_op m i x : 
+    dom ({[ i := x ]} ⋅ m) = {[i]} ∪ dom m.
+  Proof. rewrite dom_op; set_solver. Qed.
+
+  Lemma dom_singleton_op_Some m i x : 
+    is_Some (m !! i) → dom ({[ i := x ]} ⋅ m) = dom m.
+  Proof. rewrite -elem_of_dom dom_op; set_solver. Qed.
+End extra.
