lib/zrange.v
@@ -1,0 +1,77 @@
+From iris.algebra Require Import gset.
+
+
+Section zrange.
+  Local Open Scope Z.
+
+  Fixpoint zrange_gap (l: Z) (gap : nat) : gset Z :=
+    match gap with
+    | O => ∅
+    | S n => 
+      match n with
+      | O => ∅
+      | S _ => {[l + n]} ∪ (zrange_gap l n)
+      end
+    end.
+  Lemma zrange_gap_spec m l gap:
+    m ∈ zrange_gap l gap ↔ l < m < l + gap.
+  Proof.
+    destruct gap as [|gap]. { split; intros; last lia; done. }
+    induction gap as [|gap IH]. { split; intros; last lia; done. }
+    rewrite elem_of_union; split.
+    + intros [Hsing|Hrange].
+      - rewrite elem_of_singleton in Hsing; lia.
+      - rewrite IH in Hrange; lia.
+    + replace (l + S (S gap)) with (Z.succ (l + S gap)) by lia.
+      intros (?&Hle); apply Zlt_succ_le, Zle_lt_or_eq in Hle as [?|?].
+      - right; rewrite IH; lia.
+      - left; rewrite elem_of_singleton //.
+  Qed.
+
+  Definition zrange (l r: Z) : gset Z := 
+    zrange_gap l (Z.to_nat (r - l)).
+  Lemma zrange_spec m l r:
+    m ∈ zrange l r ↔ l < m < r.
+  Proof. rewrite /zrange zrange_gap_spec; lia. Qed.
+  Lemma zrange_disj S l r:
+    S ## zrange l r ↔ ∀ m, l < m < r → m ∉ S.
+  Proof. pose proof zrange_spec; set_solver. Qed.
+  Lemma zrange_disj_l l r:
+    {[l]} ## zrange l r.
+  Proof. intros ?; rewrite zrange_spec elem_of_singleton; lia. Qed.
+  Lemma zrange_disj_r l r:
+    zrange l r ## {[r]}.
+  Proof. intros ?; rewrite zrange_spec elem_of_singleton; lia. Qed.
+  Lemma zrange_disj_m m l r:
+    zrange l m ## zrange m r.
+  Proof. intros ?; do 2 rewrite zrange_spec; lia. Qed.
+  Lemma zrange_split m l r:
+    l < m < r → zrange l r = zrange l m ∪ {[m]} ∪ zrange m r.
+  Proof.
+    intros Hm; rewrite set_eq; intros m'; split.
+    + intros Hm'%zrange_spec.
+      destruct (Ztrichotomy_inf m' m) as [[Hlt|<-]|Hgt].
+      - apply elem_of_union_l, elem_of_union_l, zrange_spec; lia.
+      - by apply elem_of_union_l, elem_of_union_r, elem_of_singleton.
+      - apply elem_of_union_r, zrange_spec; lia.
+    + rewrite ?elem_of_union elem_of_singleton ?zrange_spec; intros [[Hlt|Heq]|Hgt]; lia.
+  Qed.
+End zrange.
+
+Section ZRange.
+  Local Open Scope Z.
+
+  Definition ZRange (l r: Z) : gset_disj Z := 
+    if decide(l < r) then GSet (zrange l r) else GSetBot.
+  Lemma ZRange_disj S l r:
+    ✓ (GSet S ⋅ ZRange l r) ↔ S ## zrange l r ∧ l < r.
+  Proof. rewrite /ZRange; case_decide; first set_solver; by split; last lia. Qed.
+  Lemma ZRange_split m l r:
+    l < m < r → ZRange l r = ZRange l m ⋅ GSet {[m]} ⋅ ZRange m r.
+  Proof.
+    intros ?; rewrite /ZRange; do 3 (case_decide; last lia).
+    rewrite (zrange_split m) // gset_disj_union; last apply zrange_disj_r.
+    rewrite gset_disj_union // disjoint_union_l.
+    split; first apply zrange_disj_m; apply zrange_disj_l.
+  Qed.
+End ZRange.
